src/Step.hs
@@ -10,10 +10,22 @@ eq_decide :: (EqDec a1) -> a1 -> a1 -> Prelude.Bool
 eq_decide eqDec =
   eqDec
 
+data Lambda t =
+   Build_Lambda (t -> t -> t) ((t -> t) -> t)
+
+lam :: (Lambda a1) -> (a1 -> a1) -> a1
+lam lambda =
+  case lambda of {
+   Build_Lambda _ lam0 -> lam0}
+
 data Term v =
    Var v
  | Pass (Term v) (Term v)
- | Lam (v -> Term v)
+ | Lam_ (v -> Term v)
+
+term_lambda :: Lambda (Term a1)
+term_lambda =
+  Build_Lambda (\x x0 -> Pass x x0) (\f -> Lam_ (\x -> f (Var x)))
 
 type Store v = v -> Term v
 
@@ -31,11 +43,6 @@ head f =
   case f of {
    Build_font head0 _ _ -> head0}
 
-right :: (Font a1) -> Font a1
-right f =
-  case f of {
-   Build_font _ _ right0 -> right0}
-
 data Stack v =
    Hole
  | Lpass (Stack v) (Term v)
@@ -44,7 +51,7 @@ type Heap v = [] ((,) v (Term v))
 
 arbitrary :: Term a1
 arbitrary =
-  Lam (\x -> Var x)
+  lam term_lambda (\x -> x)
 
 lookup :: (EqDec a1) -> (Heap a1) -> Store a1
 lookup h hp =
@@ -61,9 +68,10 @@ go h fnt s k e =
   case e of {
    Var x -> Prelude.Just ((,) ((,) s k) (lookup h s x));
    Pass e0 e1 -> Prelude.Just ((,) ((,) s (Lpass k e1)) e0);
-   Lam f ->
+   Lam_ f ->
     case k of {
      Hole -> Prelude.Nothing;
      Lpass k' e0 ->
-      let {x = head fnt} in go h (right fnt) ((:) ((,) x e0) s) k' (f x)}}
+      let {x = head fnt} in
+      Prelude.Just ((,) ((,) ((:) ((,) x e0) s) k') (f x))}}
 
